Semantics/Imp/Structural.lean
@@ -4,29 +4,29 @@ import Semantics.ReflTransRel
 namespace Com
 namespace Structural
 
-inductive step: Config → Config → Prop where
+inductive small_step: Config → Config → Prop where
   | assₛ:
-    step (ass₁ v a, s) (skip₁, s[v ← a s])
+    small_step (ass₁ v a, s) (skip₁, s[v ← a s])
 
   | cat₀ₛ:
-    step (skip₁++c, s) (c, s)
+    small_step (skip₁++c, s) (c, s)
 
-  | catₙₛ (h: step (c₁, s₁) (c₂, s₂)):
-    step (c₁++c₃, s₁) (c₂++c₃, s₂)
+  | catₙₛ (h: small_step (c₁, s₁) (c₂, s₂)):
+    small_step (c₁++c₃, s₁) (c₂++c₃, s₂)
 
   | ifₛ:
-    step (if b then c₁ else c₂ end, s) (bif b s then c₁ else c₂, s)
+    small_step (if b then c₁ else c₂ end, s) (bif b s then c₁ else c₂, s)
 
   | whileₛ:
-    step (while b loop c end, s)
+    small_step (while b loop c end, s)
           (bif b s then c++while b loop c end else skip₁, s)
 
-infixl:10 " =>ₛ " => step
+infixl:10 " =>ₛ " => small_step
 
 private example:
   ([|x := 0; while x ≤ 2 loop x := x + 1 end|], s₀) =>ₛ
       ([|skip; while x ≤ 2 loop x := x + 1 end|], s₀["x" ← 0]) :=
-  step.catₙₛ step.assₛ
+  small_step.catₙₛ small_step.assₛ
 
 theorem cat_eq:
   ((c₁++c₃, s₁) =>ₛ conf)
@@ -34,11 +34,11 @@ theorem cat_eq:
       ∨ (c₁ = skip₁ ∧ conf = (c₃, s₁))) :=
   propext {
     mp := λ hmp ↦ match hmp with
-      | step.cat₀ₛ => Or.inr ⟨rfl, rfl⟩
-      | step.catₙₛ h => Or.inl ⟨_, _, h, rfl⟩,
+      | small_step.cat₀ₛ => Or.inr ⟨rfl, rfl⟩
+      | small_step.catₙₛ h => Or.inl ⟨_, _, h, rfl⟩,
     mpr := λ hmpr ↦ match hmpr with
-      | Or.inl ⟨_c₂, _s₂, h₁, h₂⟩ => h₂ ▸ step.catₙₛ h₁
-      | Or.inr ⟨h₁, h₂⟩ => h₁ ▸ h₂ ▸ step.cat₀ₛ
+      | Or.inl ⟨_c₂, _s₂, h₁, h₂⟩ => h₂ ▸ small_step.catₙₛ h₁
+      | Or.inr ⟨h₁, h₂⟩ => h₁ ▸ h₂ ▸ small_step.cat₀ₛ
   }
 
 theorem cond_eq:
@@ -46,14 +46,14 @@ theorem cond_eq:
     = (b s ∧ conf = (c₁, s) ∨ b s = false ∧ conf = (c₂, s)) :=
   propext {
     mp := λ hmp ↦ match hb: b s with
-      | false => match hmp with | step.ifₛ => Or.inr ⟨rfl, hb ▸ rfl⟩
-      | true => match hmp with | step.ifₛ => Or.inl ⟨rfl, hb ▸ rfl⟩,
+      | false => match hmp with | small_step.ifₛ => Or.inr ⟨rfl, hb ▸ rfl⟩
+      | true => match hmp with | small_step.ifₛ => Or.inl ⟨rfl, hb ▸ rfl⟩,
     mpr := λ hmpr ↦
       let hss: conf = (bif b s then c₁ else c₂, s) :=
         match hb: b s with
         | true => match hb ▸ hmpr with | Or.inl ⟨_, h₂⟩ => h₂
         | false => match hb ▸ hmpr with | Or.inr ⟨_, h₂⟩ => h₂
-      hss ▸ step.ifₛ
+      hss ▸ small_step.ifₛ
   }
 
 theorem cond_false (hb: b s₁ = false):
@@ -64,28 +64,28 @@ theorem cond_false (hb: b s₁ = false):
     mpr := λ hmpr ↦ cond_eq ▸ Or.inr ⟨hb, hmpr⟩
   }
 
-infixl:10 " =>ₛ* " => RTL step
+infixl:10 " =>ₛ* " => RTL small_step
 
 theorem star.demo₂:
   ([|x := 2; while 0 ≤ x loop x := x + 1 end|], s₀) =>ₛ*
       ([|while 0 ≤ x loop x := x + 1 end|], s₀["x" ← 2]) :=
-  RTL.head (step.catₙₛ step.assₛ) (RTL.head step.cat₀ₛ RTL.refl)
+  RTL.head (small_step.catₙₛ small_step.assₛ) (RTL.head small_step.cat₀ₛ RTL.refl)
 
 theorem star.cat_skip_cat
   (hc₁: (c₁, s₁) =>ₛ* (skip₁, s₂)):
   (c₁++c₂, s₁) =>ₛ* (skip₁++c₂, s₂) :=
-  RTL.lift (λ (c₁, s) ↦ (c₁++c₂, s)) (λ h ↦ step.catₙₛ h) hc₁
+  RTL.lift (λ (c₁, s) ↦ (c₁++c₂, s)) (λ h ↦ small_step.catₙₛ h) hc₁
 
 theorem star.cat
   (hc₁: (c₁, s₁) =>ₛ* (skip₁, s₂))
   (hc₂: (c₂, s₂) =>ₛ* (skip₁, s₃)):
   (c₁++c₂, s₁) =>ₛ* (skip₁, s₃) :=
-  RTL.trans (cat_skip_cat hc₁) (RTL.trans (RTL.single step.cat₀ₛ) hc₂)
+  RTL.trans (cat_skip_cat hc₁) (RTL.trans (RTL.single small_step.cat₀ₛ) hc₂)
 
 theorem star.cat_no_influence
   (hc₁: (c₁, s) =>ₛ* (skip₁, s₁)):
   (c₁++c₂, s) =>ₛ* (c₂, s₁) :=
-  RTL.trans (cat_skip_cat hc₁) (RTL.single step.cat₀ₛ)
+  RTL.trans (cat_skip_cat hc₁) (RTL.single small_step.cat₀ₛ)
 
 end Structural
 end Com
