Semantics/Imp/Equivalence.lean
@@ -8,30 +8,30 @@ theorem Structural.from_natural
   (hconf: conf ==>ₙ s₂): conf =>ₛ* (skip₁, s₂) := by
   induction hconf with
   | skipₙ => exact RTL.refl
-  | assₙ => exact RTL.single step.assₛ
+  | assₙ => exact RTL.single small_step.assₛ
   | catₙ _ _ _ ihc₁ ihc₂ => exact star.cat ihc₁ ihc₂
-  | if₁ₙ hb _ ih => exact RTL.head step.ifₛ (hb ▸ ih)
-  | if₀ₙ hb _ ih => exact RTL.head step.ifₛ (hb ▸ ih)
+  | if₁ₙ hb _ ih => exact RTL.head small_step.ifₛ (hb ▸ ih)
+  | if₀ₙ hb _ ih => exact RTL.head small_step.ifₛ (hb ▸ ih)
   | while₁ₙ _ hb _ _ ihc ihw =>
-    exact RTL.head step.whileₛ $ RTL.trans (hb ▸ star.cat ihc ihw) RTL.refl
+    exact RTL.head small_step.whileₛ $ RTL.trans (hb ▸ star.cat ihc ihw) RTL.refl
   | while₀ₙ hb =>
-    exact RTL.head step.whileₛ $ hb ▸ RTL.refl
+    exact RTL.head small_step.whileₛ $ hb ▸ RTL.refl
 
 theorem Natural.from_structural_step
   (hconf₁: conf₁ =>ₛ conf₂) (hconf₂: conf₂ ==>ₙ s₂): conf₁ ==>ₙ s₂ := by
   induction hconf₁ generalizing s₂ with
-  | assₛ => exact (skip_eq.mp hconf₂) ▸ step.assₙ
-  | cat₀ₛ => exact step.catₙ _ step.skipₙ hconf₂
+  | assₛ => exact (skip_eq.mp hconf₂) ▸ big_step.assₙ
+  | cat₀ₛ => exact big_step.catₙ _ big_step.skipₙ hconf₂
   | catₙₛ _ ih =>
     match hconf₂ with
-    | step.catₙ s₂ hc₁ hc₂ => exact step.catₙ s₂ (ih hc₁) hc₂
+    | big_step.catₙ s₂ hc₁ hc₂ => exact big_step.catₙ s₂ (ih hc₁) hc₂
   | ifₛ => exact if_eq' ▸ hconf₂
   | whileₛ => rw [loop_unfold]; exact if_eq' ▸ hconf₂
 
 theorem Natural.from_structural
   (hconf: conf =>ₛ* (skip₁, s₂)): conf ==>ₙ s₂ := by
   induction hconf using RTL.head_induction_on with
-  | refl => exact step.skipₙ
+  | refl => exact big_step.skipₙ
   | head hsingle _ hs₂ => exact from_structural_step hsingle hs₂
 
 theorem structural_eq_natural:
@@ -68,23 +68,23 @@ theorem Natural.from_denote
   | skip₁ =>
     intro hmp
     rw [denote, SFun.mem_id] at hmp
-    exact hmp ▸ step.skipₙ
+    exact hmp ▸ big_step.skipₙ
   | ass₁ =>
     intro hmp
     rw [denote.eq_def, Set.mem_comprehend] at hmp
     simp only at hmp
-    exact hmp ▸ step.assₙ
+    exact hmp ▸ big_step.assₙ
   | cat₁ _ _ ih₁ ih₂ =>
     intro ⟨s₂, h₁, h₂⟩
-    exact step.catₙ s₂ (ih₁ h₁) (ih₂ h₂)
+    exact big_step.catₙ s₂ (ih₁ h₁) (ih₂ h₂)
   | if₁ _ _ _ ih₁ ih₂ =>
     intro hmp
     match hmp with
     | Or.inl ⟨h₁, hb⟩ =>
-      exact step.if₁ₙ hb (ih₁ h₁)
+      exact big_step.if₁ₙ hb (ih₁ h₁)
     | Or.inr ⟨h₁, hb⟩ =>
       simp only [Set.mem_comprehend, Bool.not_eq_true] at hb
-      exact step.if₀ₙ hb (ih₂ h₁)
+      exact big_step.if₀ₙ hb (ih₂ h₁)
   | while₁ b c ih =>
     suffices
       ⟦while b loop c end⟧ ⊆ {(s₁, s₃) | (while b loop c end, s₁) ==>ₙ s₃} by
@@ -94,11 +94,11 @@ theorem Natural.from_denote
     intro ⟨_, _⟩ hmp
     match hmp with
     | Or.inl ⟨⟨s₂, h₁, h₂⟩, hb⟩ =>
-      exact step.while₁ₙ s₂ hb (ih h₁) h₂
+      exact big_step.while₁ₙ s₂ hb (ih h₁) h₂
     | Or.inr ⟨hid, hb⟩ =>
       simp only [Set.mem_comprehend, Bool.not_eq_true] at hb
       rw [SFun.mem_id] at hid
-      exact hid ▸ step.while₀ₙ hb
+      exact hid ▸ big_step.while₀ₙ hb
 
 theorem natural_eq_denote: ((s₁, s₂) ∈ ⟦c⟧) = ((c, s₁) ==>ₙ s₂) :=
   propext ⟨Natural.from_denote, denote.from_natural⟩
